

5

1. An equation of the line tangent to the graph of  $y = \frac{2x+3}{3x-2}$  at the point (1, 5) is
- (A)  $13x-y=8$   
(B)  $13x+y=18$   
(C)  $x-13y=64$   
(D)  $x+13y=66$   
(E)  $-2x+3y=13$
2. If  $f(x) = \frac{3x-2}{2x+3}$ , then  $f'(x) =$
- (A)  $-\frac{13}{(2x+3)^2}$   
(B)  $\frac{3}{(2x+3)^2}$   
(C)  $\frac{5}{(2x+3)^2}$   
(D)  $\frac{13}{(2x+3)^2}$   
(E)  $\frac{12x+5}{(2x+3)^2}$
3. If  $y = \frac{2x+3}{3x+2}$ , then  $\frac{dy}{dx} =$
- (A)  $\frac{12x+13}{(3x+2)^2}$   
(B)  $\frac{12x-13}{(3x+2)^2}$   
(C)  $\frac{5}{(3x+2)^2}$   
(D)  $\frac{-5}{(3x+2)^2}$   
(E)  $\frac{2}{3}$
4. If  $y = \frac{\ln x}{x}$ , then  $\frac{dy}{dx} =$
- (A)  $\frac{1}{x}$   
(B)  $\frac{1}{x^2}$   
(C)  $\frac{\ln x - 1}{x^2}$   
(D)  $\frac{1 - \ln x}{x^2}$   
(E)  $\frac{1 + \ln x}{x^2}$
5. What is the instantaneous rate of change at  $x=2$  of the function  $f$  given by  $f(x) = \frac{x^2-2}{x-1}$  ?

5

- (A) -2
- (B)  $\frac{1}{6}$
- (C)  $\frac{1}{2}$
- (D) 2
- (E) 6

6. If  $f(x) = \frac{5-x}{x^3+2}$ , then  $f'(x) =$

- (A)  $\frac{-4x^3+15x^2-2}{(x^3+2)^2}$
- (B)  $\frac{-2x^3+15x^2+2}{(x^3+2)^2}$
- (C)  $\frac{2x^3-15x^2-2}{(x^3+2)^2}$
- (D)  $\frac{4x^3-15x^2+2}{(x^3+2)^2}$

7. If  $y = \tan x - \cot x$ , then  $dy/dx =$

- (A)  $\sec x \csc x$
- (B)  $\sec x - \csc x$
- (C)  $\sec x + \csc x$
- (D)  $\sec^2 x - \csc^2 x$
- (E)  $\sec^2 x + \csc^2 x$

8.  $\frac{d}{dx} \left( \frac{x+1}{x^2+1} \right) =$

- (A)  $\frac{x^2+2x-1}{(x^2+1)^2}$
- (B)  $\frac{-x^2-2x+1}{x^2+1}$
- (C)  $\frac{-x^2-2x+1}{(x^2+1)^2}$
- (D)  $\frac{3x^2+2x+1}{(x^2+1)^2}$
- (E)  $\frac{1}{2x}$

9. If  $f(x) = \frac{x^2+3x+2}{x+3}$ , then  $f'(x) =$

- (A)  $2x + 3$
- (B)  $\frac{-x^2-6x-7}{(x+3)^2}$
- (C)  $\frac{x^2+6x+7}{(x+3)^2}$
- (D)  $\frac{x^2+12x+11}{(x+3)^2}$
- (E)  $\frac{3x^2+12x+11}{(x+3)^2}$

5

10. The function  $f$  is defined by  $f(x) = \frac{x}{x+2}$ . What points  $(x, y)$  on the graph of  $f$  have the property that the line tangent to  $f$  at  $(x, y)$  has slope  $\frac{1}{2}$ ?
- (A)  $(0, 0)$  only  
(B)  $(\frac{1}{2}, \frac{1}{5})$  only  
(C)  $(0, 0)$  and  $(-4, 2)$   
(D)  $(0, 0)$  and  $(4, \frac{2}{3})$   
(E) There are no such points.
11. If  $f(x) = \frac{5-x}{x^3+2}$ , then  $f'(x) =$
- (A)  $\frac{-4x^3+15x^2-2}{(x^3+2)^2}$   
(B)  $\frac{-2x^3+15x^2+2}{(x^3+2)^2}$   
(C)  $\frac{2x^3-15x^2-2}{(x^3+2)^2}$   
(D)  $\frac{4x^3-15x^2+2}{(x^3+2)^2}$
12. What is the slope of the line tangent to the graph of  $y = \frac{x^2-2}{x^2+1}$  when  $x = 1$ ?
- (A)  $-\frac{3}{2}$   
(B)  $-\frac{1}{2}$   
(C)  $\frac{1}{2}$   
(D) 1  
(E)  $\frac{3}{2}$
- 13.

$x$	$f(x)$	$f'(x)$	$g(x)$	$g'(x)$
0	3	4	2	$\pi$

The table above gives values of the differentiable functions  $f$  and  $g$  and their derivatives at  $x = 0$ . If  $h(x) = \frac{f(x)}{g(x)}$ , what is the value of  $h'(0)$ ?

- (A)  $\frac{8-3\pi}{4}$   
(B)  $\frac{3\pi-8}{4}$   
(C)  $\frac{4}{\pi}$   
(D)  $\frac{2-3\pi}{2}$   
(E)  $\frac{8+3\pi}{4}$

5

14.

$f(3)$	$g(3)$	$f'(3)$	$g'(3)$
-1	2	5	-2

The table above gives values for the functions  $f$  and  $g$  and their derivatives at  $x = 3$ . Let  $k$  be the function given by  $k(x) = \frac{f(x)}{g(x)}$ , where  $g(x) \neq 0$ . What is the value of  $k'(3)$ ?

- (A)  $-\frac{5}{2}$   
(B) -2  
(C) 2  
(D) 3  
(E) 8

15. Given that  $3x - \tan y = 4$ , what is  $\frac{dy}{dx}$  in terms of  $y$ ?

- (A)  $\frac{dy}{dx} = 3\sin^2 y$   
(B)  $\frac{dy}{dx} = 3\cos^2 y$   
(C)  $\frac{dy}{dx} = 3 \cos y \cot y$   
(D)  $\frac{dy}{dx} = \frac{3}{1+9y^2}$

16. Which of the following correctly shows the derivation of  $\frac{d}{dx}(\sec x)$ ?

- (A)  $\frac{d}{dx}(\sec x) = \frac{d}{dx}\left(\frac{1}{\cos x}\right) = \frac{1}{\frac{d}{dx}(\cos x)} = \frac{1}{\sin x}$   
(B)  $\frac{d}{dx}(\sec x) = \frac{d}{dx}\left(\frac{1}{\cos x}\right) = \frac{1}{\frac{d}{dx}(\cos x)} = \frac{1}{-\sin x}$   
(C)  $\frac{d}{dx}(\sec x) = \frac{d}{dx}\left(\frac{1}{\cos x}\right) = \frac{\frac{d}{dx}(1) \cdot \cos x - 1 \cdot \frac{d}{dx}(\cos x)}{(\cos x)^2} = \frac{0 \cdot \cos x - 1 \cdot (-\sin x)}{(\cos x)^2}$   
(D)  $\frac{d}{dx}(\sec x) = \frac{d}{dx}\left(\frac{1}{\cos x}\right) = \frac{\frac{d}{dx}(1) \cdot \cos x + 1 \cdot \frac{d}{dx}(\cos x)}{(\cos x)^2} = \frac{0 \cdot \cos x + 1 \cdot (-\sin x)}{(\cos x)^2}$

17.  $\frac{d}{dx}(\cot x) =$

- (A)  $-\tan x$   
(B)  $-\csc^2 x$   
(C)  $\csc x$   
(D)  $\sec^2 x$

18. If  $f(x) = \tan x$ , then  $\lim_{x \rightarrow \frac{\pi}{4}} \frac{f(x) - f(\frac{\pi}{4})}{x - \frac{\pi}{4}}$  is

5

- (A) 0
- (B)  $\tan\left(\frac{\pi}{4}\right)$
- (C)  $\sec^2\left(\frac{\pi}{4}\right)$
- (D) nonexistent

19. Which of the following correctly shows the derivation of  $\frac{d}{dx}(\cot x)$ ?

- (A)  $\frac{d}{dx}(\cot x) = \frac{d}{dx}\left(\frac{1}{\tan x}\right) = \frac{1}{\frac{d}{dx}(\tan x)} = \frac{-1}{\sec^2 x}$
- (B)  $\frac{d}{dx}(\cot x) = \frac{d}{dx}\left(\frac{1}{\tan x}\right) = \frac{1}{\frac{d}{dx}(\tan x)} = \frac{1}{\sec^2 x}$
- (C)  $\frac{d}{dx}(\cot x) = \frac{d}{dx}\left(\frac{1}{\tan x}\right) = \frac{\tan x \frac{d}{dx}(1) - 1 \cdot \frac{d}{dx}(\tan x)}{\tan^2 x} = \frac{(\tan x) \cdot 0 - \sec^2 x}{\tan^2 x} = -\frac{\sec^2 x}{\tan^2 x}$
- (D)  $\frac{d}{dx}(\cot x) = \frac{d}{dx}\left(\frac{1}{\tan x}\right) = \frac{\tan x \frac{d}{dx}(1) + 1 \cdot \frac{d}{dx}(\tan x)}{\tan^2 x} = \frac{\tan x \cdot 0 + \sec^2 x}{\tan^2 x} = \frac{\sec^2 x}{\tan^2 x}$

20.  $\frac{d}{dx}(\cos x \tan x) =$

- (A)  $\sec x + \sin x \tan x$
- (B)  $\cos x$
- (C)  $-\sin x \sec^2 x$
- (D)  $\sin x$

21. If  $f(x) = \sec x$ , then  $\lim_{x \rightarrow \frac{\pi}{3}} \frac{f(x) - f(\frac{\pi}{3})}{x - \frac{\pi}{3}}$  is

- (A) 0
- (B)  $\sec\left(\frac{\pi}{3}\right)$
- (C)  $\sec\left(\frac{\pi}{3}\right) \tan\left(\frac{\pi}{3}\right)$
- (D) nonexistent

22.  $\lim_{x \rightarrow 0} \frac{\sin x}{e^x - 1}$  is

- (A) 1
- (B)  $\frac{1}{e}$
- (C) 0
- (D) nonexistent

5

23.

$x$	$f(x)$	$f'(x)$	$g(x)$	$g'(x)$
2	-3	$\frac{1}{2}$	-3	2

The table above gives values of the differentiable functions  $f$  and  $g$  and their derivatives at  $x = 2$ . If  $h(x) = \frac{4f(x)}{g(x)+1}$ , then  $h'(2) =$

- (A) -10  
(B) -7  
(C) 1  
(D) 5

24.

$x$	$f(x)$	$f'(x)$	$f''(x)$	$g(x)$	$g'(x)$	$g''(x)$
2	4	-3	3	-2	5	1

The table above gives values of the twice-differentiable functions  $f$  and  $g$  and their derivatives at  $x = 2$ . If  $h$  is the function defined by  $h(x) = \frac{f'(x)}{g(x)}$ , what is the value of  $h'(2)$ ?

- (A)  $\frac{9}{4}$   
(B)  $\frac{3}{5}$   
(C)  $-\frac{3}{2}$   
(D)  $-\frac{21}{4}$

25. If  $f(x) = x^2 + 4x - 2$ ,  $g(x) = 4x + 2$ , and  $h(x) = \frac{f(x)}{g(x)}$ , then  $h'(1) =$

- (A)  $-\frac{2}{3}$   
(B)  $\frac{2}{3}$   
(C)  $\frac{4}{3}$   
(D)  $\frac{3}{2}$

26.

$x$	$f(x)$	$f'(x)$	$g(x)$	$g'(x)$
2	5	3	2	4

The table shown gives values of the differentiable functions  $f$  and  $g$  and their derivatives at  $x = 2$ . If  $h(x) = \frac{f(x)}{g(x)}$ , what is the value of  $h'(2)$ ?

5

- (A)  $-\frac{7}{2}$   
(B)  $-\frac{7}{8}$   
(C)  $\frac{3}{4}$   
(D)  $\frac{13}{2}$

27. If  $y = \frac{x^3}{x+2}$ , then  $\frac{dy}{dx} =$

- (A)  $3x^2$   
(B)  $\frac{-2x^3-6x^2}{(x+2)^2}$   
(C)  $\frac{2x^3+6x^2}{(x+2)^2}$   
(D)  $\frac{4x^3+6x^2}{(x+2)^2}$

28.

$x$	$f(x)$	$g(x)$	$f'(x)$	$g'(x)$
2	-1	-4	5	3

The table shown gives values of functions  $f$ ,  $g$ ,  $f'$ , and  $g'$  at  $x = 2$ . If  $h(x) = \frac{f(x)}{g(x)}$ , then  $h'(2) =$

- (A)  $-\frac{23}{16}$   
(B)  $-\frac{17}{16}$   
(C)  $-\frac{11}{16}$   
(D)  $\frac{5}{3}$

29. If  $f(x) = \frac{\sin x}{e^x}$ , then  $f'(x) =$

- (A)  $\frac{-\cos x - \sin x}{e^x}$   
(B)  $\frac{\cos x - \sin x}{e^x}$   
(C)  $\frac{\sin x - \cos x}{e^x}$   
(D)  $\frac{\cos x + \sin x}{e^x}$

30. Let  $f$  be a differentiable function such that  $f(9) = 18$  and  $f'(9) = 7$ . If  $g$  is the function defined by  $g(x) = \frac{f(x)}{\sqrt{x}}$ , what is the value of  $g'(9)$ ?

- (A) 2  
(B)  $\frac{7}{3}$   
(C)  $\frac{8}{3}$   
(D) 42

31. If  $f(x) = \frac{\cos x}{\ln x}$ , then  $f'(x) =$

5

- (A)  $\frac{x \sin x \ln x - \cos x}{x(\ln x)^2}$
- (B)  $\frac{-x \sin x \ln x - \cos x}{x(\ln x)^2}$
- (C)  $-x \sin x$
- (D)  $\frac{-x \sin x \ln x + \cos x}{x(\ln x)^2}$

32. Let  $f$  be a differentiable function such that  $f(8) = 2$  and  $f'(8) = 5$ . If  $g$  is the function defined by  $g(x) = \frac{f(x)}{\sqrt[3]{x}}$ , what is the value of  $g'(8)$ ?

- (A)  $\frac{59}{24}$
- (B)  $\frac{5}{2}$
- (C)  $\frac{61}{24}$
- (D) 60

33.

$x$	$f(x)$	$f'(x)$	$g(x)$	$g'(x)$
0	4	$\frac{1}{2}$	-2	$\frac{3}{2}$

The table above gives values of the differentiable functions  $f$  and  $g$  and their derivatives at  $x = 0$ . If  $h(x) = \frac{6f(x)}{g(x)-1}$ , then  $h'(0) =$

- (A) 15
- (B) 3
- (C) 2
- (D) -5